

1 Pauli Gate

$$XY = iZ \quad XZ = -iY \quad YZ = iX \quad (1)$$

2 UCC

$$U(\theta) = e^{\hat{T}(\theta) - \hat{T}(\theta)^\dagger} \quad (2)$$

$$\hat{T} = \theta \hat{a}_i^\dagger \hat{a}_j^\dagger \hat{a}_k \hat{a}_l \quad i > j > k > l \quad (3)$$

$$U(\theta) = e^{\theta(\hat{a}_i^\dagger \hat{a}_j^\dagger \hat{a}_k \hat{a}_l - \hat{a}_l^\dagger \hat{a}_k^\dagger \hat{a}_j \hat{a}_i)} \quad (4)$$

Now plug in the jordan wigner transformation.

$$\hat{a}_i^\dagger = I^{\otimes i} \otimes \frac{1}{2}(X - iY) \otimes Z^{\otimes N-i-1} \quad (5)$$

$$\hat{a}_i = I^{\otimes i} \otimes \frac{1}{2}(X + iY) \otimes Z^{\otimes N-i-1} \quad (6)$$

where N is the number of qbit. $i = [0, \dots, N-1]$. Now we calculate

$$a_i^\dagger a_j^\dagger a_k a_l - a_l^\dagger a_k^\dagger a_j a_i \quad (7)$$

Let's from smaller term and assume $i > j$.

$$a_i^\dagger a_j^\dagger = [I^{\otimes i} \otimes \frac{1}{2}(X - iY) \otimes Z^{\otimes N-i-1}] [I^{\otimes j} \otimes \frac{1}{2}(X - iY) \otimes Z^{\otimes N-j-1}] \quad (8)$$

$$= [I^{\otimes j} \otimes \frac{1}{2}(X_j - iY_j) \otimes_{a=j+1}^{i-1} Z_a \otimes \frac{1}{2}(X_i - iY_i) Z_i \otimes I^{\otimes N-i-1}] \quad (9)$$

$$= [I^{\otimes j} \otimes \frac{1}{2}(X_j - iY_j) \otimes_{a=j+1}^{i-1} Z_a \otimes \frac{1}{2}(-iY_i + X_i) \otimes I^{\otimes N-i-1}] \quad (10)$$

$$= [I^{\otimes j} \otimes \frac{1}{2}(X_j - iY_j) \otimes_{a=j+1}^{i-1} Z_a \otimes \frac{1}{2}(X_i - iY_i) \otimes I^{\otimes N-i-1}] \quad (11)$$

Now annihilation term is $k > l$

$$a_k a_l = [I^{\otimes k} \otimes \frac{1}{2}(X_k + iY_k) \otimes Z^{\otimes N-k-1}] [I^{\otimes l} \otimes \frac{1}{2}(X_l + iY_l) \otimes Z^{\otimes N-l-1}] \quad (12)$$

$$= [I^{\otimes l} \otimes \frac{1}{2}(X_l + iY_l) \otimes_{a=l+1}^{k-1} Z_a \otimes \frac{1}{2}(X_k + iY_k) Z_k \otimes I^{\otimes N-k-1}] \quad (13)$$

$$= [I^{\otimes l} \otimes \frac{1}{2}(X_l + iY_l) \otimes_{a=l+1}^{k-1} Z_a \otimes \frac{1}{2}(-iY_k - X_k) \otimes I^{\otimes N-k-1}] \quad (14)$$

$$= -[I^{\otimes l} \otimes \frac{1}{2}(X_l + iY_l) \otimes_{a=l+1}^{k-1} Z_a \otimes \frac{1}{2}(X_k + iY_k) \otimes I^{\otimes N-k-1}] \quad (15)$$

Now we combine this two terms, $i > j > k > l$

$$\begin{aligned} a_i^\dagger a_j^\dagger a_k a_l &= [I^{\otimes j} \otimes \frac{1}{2}(X_j - iY_j) \otimes_{a=j+1}^{i-1} Z_a \otimes \frac{1}{2}(X_i - iY_i) \otimes I^{\otimes N-i-1}] \\ &\quad \times [-I^{\otimes l} \otimes \frac{1}{2}(X_l + iY_l) \otimes_{a=l+1}^{k-1} Z_a \otimes \frac{1}{2}(X_k + iY_k) \otimes I^{\otimes N-k-1}] \\ &= -[I^{\otimes l} \otimes \frac{1}{2}(X_l + iY_l) \otimes_{a=l+1}^{k-1} Z_a \otimes \frac{1}{2}(X_k + iY_k) \otimes_{b=k+1}^j I_b \otimes \frac{1}{2}(X_j - iY_j) \otimes_{c=j+1}^{i-1} Z_c \otimes \frac{1}{2}(X_i - iY_i) \otimes I^{\otimes N-i-1}] \\ &= -\otimes_{a=l+1}^{k-1} Z_a \otimes_{b=j+1}^{i-1} Z_b \otimes \frac{1}{2}(X_l + iY_l) \otimes \frac{1}{2}(X_k + iY_k) \otimes \frac{1}{2}(X_j - iY_j) \otimes \frac{1}{2}(X_i - iY_i) \\ &= -\frac{1}{16} \otimes_{a=l+1}^{k-1} Z_a \otimes_{b=j+1}^{i-1} Z_b (X_l + iY_l)(X_k + iY_k)(X_j - iY_j)(X_i - iY_i) \end{aligned}$$

There are 16 pauli string, but we calculate the conjugate term Now with $i > j > k > l$

$$a_l^\dagger a_k^\dagger a_j a_i = a_k^\dagger a_l^\dagger a_i a_j \quad (16)$$

$$a_l^\dagger a_k^\dagger a_j a_i = [I^{\otimes l} \otimes \frac{1}{2}(X_l - iY_l) \otimes_{a=l+1}^{k-1} Z_a \otimes \frac{1}{2}(X_k - iY_k) \otimes I^{\otimes N-k-1}] \quad (17)$$

$$\times [-I^{\otimes j} \otimes \frac{1}{2}(X_j + iY_j) \otimes_{a=j+1}^{i-1} Z_a \otimes \frac{1}{2}(X_i + iY_i) \otimes I^{\otimes N-i-1}] \quad (18)$$

$$= -\frac{1}{16} \otimes_{a=l+1}^{k-1} Z_a \otimes_{b=j+1}^{i-1} Z_b (X_l - iY_l)(X_k - iY_k)(X_j + iY_j)(X_i + iY_i) \quad (19)$$

	$X_j X_i(1)$	$X_j Y_i(-i)$	$Y_j X_i(-i)$	$Y_j Y_i(-1)$
$X_l X_k(1)$	1	-i	-i	-1
$X_l Y_k(i)$	i	1	1	-i
$Y_l X_k(i)$	i	1	1	-i
$Y_l Y_k(-1)$	-1	i	i	1

	$X_j X_i(1)$	$X_j Y_i(i)$	$Y_j X_i(i)$	$Y_j Y_i(-1)$
$X_l X_k(1)$	1	i	i	-1
$X_l Y_k(-i)$	-i	1	1	i
$Y_l X_k(-i)$	-i	1	1	i
$Y_l Y_k(-1)$	-1	-i	-i	1

Finally we want to compute $a_i^\dagger a_j^\dagger a_k a_l - a_l^\dagger a_k^\dagger a_j a_i$

We just find the coeff that are differenct. So the final result is

$$a_i^\dagger a_j^\dagger a_k a_l - a_l^\dagger a_k^\dagger a_j a_i = -\frac{1}{8}[-iX_l X_k X_j Y_i - iX_l X_k Y_j X_i] \quad (20)$$

$$iX_l Y_k X_j X_i - iX_l Y_k Y_j Y_i \quad (21)$$

$$iY_l X_k X_j X_i - iY_l X_k Y_j Y_i \quad (22)$$

$$iY_l Y_k X_j Y_i + iY_l Y_k Y_j X_i] \quad (23)$$

$$= \frac{i}{8}[X_l X_k X_j Y_i + X_l X_k Y_j X_i \quad (24)$$

$$- X_l Y_k X_j X_i + X_l Y_k Y_j Y_i \quad (25)$$

$$- Y_l X_k X_j X_i + Y_l X_k Y_j Y_i \quad (26)$$

$$- Y_l Y_k X_j Y_i - Y_l Y_k Y_j X_i] \quad (27)$$

3 Commutator

all of those eight term have the form of same two and diff two . if they diff by diff two ,that is two .if they diff by same two ,that is also two. if all diff then two by two also two.

$$[X \otimes Y, Y \otimes X] = (XY) \otimes (YX) - (YX) \otimes (XY) = (iZ) \otimes (-iZ) - (-iZ) \otimes (iZ) = 0 \quad (28)$$

so all those eight terms commute with each other.

4 CNOT -staircase construction

$$H = \frac{1}{\sqrt{2}} \begin{pmatrix} 1 & 1 \\ 1 & -1 \end{pmatrix} \quad (29)$$

$$HZH = \frac{1}{2} \begin{pmatrix} 1 & 1 \\ 1 & -1 \end{pmatrix} \begin{pmatrix} 1 & 0 \\ 0 & -1 \end{pmatrix} \begin{pmatrix} 1 & 1 \\ 1 & -1 \end{pmatrix} = \frac{1}{2} \begin{pmatrix} 1 & 1 \\ 1 & -1 \end{pmatrix} \begin{pmatrix} 1 & 1 \\ -1 & 1 \end{pmatrix} = \begin{pmatrix} 0 & 1 \\ 1 & 0 \end{pmatrix} = X \quad (30)$$

$$HH = \frac{1}{2} \begin{pmatrix} 1 & 1 \\ 1 & -1 \end{pmatrix} \begin{pmatrix} 1 & 1 \\ 1 & -1 \end{pmatrix} = I \quad (31)$$

$$e^X = e^{HZH} = H e^Z H \quad (32)$$

$$R_x(\theta) = \begin{pmatrix} \cos(\theta/2) & -i \sin(\theta/2) \\ -i \sin(\theta/2) & \cos(\theta/2) \end{pmatrix} \quad (33)$$

$$R_x(-\pi/2) = \frac{1}{\sqrt{2}} \begin{pmatrix} 1 & i \\ i & 1 \end{pmatrix} \quad R_x(\pi/2) = \frac{1}{\sqrt{2}} \begin{pmatrix} 1 & -i \\ -i & 1 \end{pmatrix} \quad (34)$$

$$R_x(-\pi/2)R_x(\pi/2) = I \quad (35)$$

$$R_x(-\pi/2)ZR_x(\pi/2) = \frac{1}{2}(1+iX)Z(1-iX) = \frac{1}{2}(1+iX)(Z-iZX) = \frac{1}{2}(1+iX)(Z-i(iY)) \quad (36)$$

$$= \frac{1}{2}(1+iX)(Z+Y) = \frac{1}{2}(Z+iXZ+Y+iXY) = Z+i(-iY)+Y+i(iZ) = Y \quad (37)$$

Now what is the quantum circuit for $i > j > k > l$

$$U(\theta) = e^{\frac{i\theta}{8} \otimes_{a=l+1}^{k-1} Z_a \otimes_{j+1}^{i-1} Z_b X_l X_k X_j Y_i} \quad (38)$$

$$U(\theta) = (HHHR_x(-\pi/2)) e^{\frac{i\theta}{8} (\otimes_{a=l}^k Z_a \otimes_{b=j}^i Z_b)} (HHHR_x(\pi/2)) \quad (39)$$